cedar-dafny/validation/subtyping.dfy
@@ -28,11 +28,11 @@ module validation.subtyping {
     }
   }
 
-  predicate subtyAttrType(a1: AttrType, a2: AttrType) {
-    subty(a1.ty, a2.ty) && (a2.isRequired ==> a1.isRequired)
+  predicate subtyAttrType(a1: AttrType, a2: AttrType, m: ValidationMode) {
+    subty(a1.ty, a2.ty, m) && (a2.isRequired ==> a1.isRequired)
   }
 
-  predicate subtyRecordType(rt1: RecordType, rt2: RecordType)
+  predicate subtyRecordType(rt1: RecordType, rt2: RecordType, m: ValidationMode)
     decreases Type.Record(rt1) , Type.Record(rt2) , 0
   {
     (rt1.isOpen() ==> rt2.isOpen()) &&
@@ -40,24 +40,28 @@ module validation.subtyping {
     rt2.attrs.Keys <= rt1.attrs.Keys &&
     // depth subtyping
     (forall k | k in rt2.attrs.Keys ::
-       subtyAttrType(rt1.attrs[k], rt2.attrs[k])) &&
+       subtyAttrType(rt1.attrs[k], rt2.attrs[k], m)) &&
     // disable width subtyping if `rt2` is closed.
-    (!rt2.isOpen() ==> rt1.attrs.Keys == rt2.attrs.Keys)
+    ((!rt2.isOpen() || m.isStrict()) ==> rt1.attrs.Keys == rt2.attrs.Keys)
   }
 
-  predicate subtyEntity(lub1: EntityLUB, lub2: EntityLUB) {
-    lub1.subset(lub2)
+  predicate subtyEntity(lub1: EntityLUB, lub2: EntityLUB, m:ValidationMode) {
+    if m.isStrict()
+    then lub1 == lub2
+    else lub1.subset(lub2)
   }
 
-  predicate subty(t1: Type, t2: Type) {
+  predicate subty(t1: Type, t2: Type, m: ValidationMode)
+    decreases t1, t2
+  {
     match (t1,t2) {
       case (Never,_) => true
       case (String,String) => true
       case (Int,Int) => true
       case (Bool(b1),Bool(b2)) => subtyBool(b1,b2)
-      case (Set(t11),Set(t21)) => subty(t11,t21)
-      case (Record(rt1),Record(rt2)) => subtyRecordType(rt1,rt2)
-      case (Entity(lub1),Entity(lub2)) => subtyEntity(lub1,lub2)
+      case (Set(t11),Set(t21)) => subty(t11,t21,m)
+      case (Record(rt1),Record(rt2)) => subtyRecordType(rt1,rt2,m)
+      case (Entity(lub1),Entity(lub2)) => subtyEntity(lub1,lub2,m)
       case (Extension(e1),Extension(e2)) => e1 == e2
       case _ => false
     }
@@ -71,40 +75,46 @@ module validation.subtyping {
     }
   }
 
-  function lubEntity(lub1: EntityLUB, lub2: EntityLUB): EntityLUB {
-    lub1.union(lub2)
+  function lubEntity(lub1: EntityLUB, lub2: EntityLUB, m: ValidationMode): Result<EntityLUB> {
+    if m.isStrict()
+    then if lub1 == lub2 then Ok(lub1.union(lub2)) else Err(LubErr(Type.Entity(lub1), Type.Entity(lub2)))
+    else Ok(lub1.union(lub2))
   }
 
-  function lubAttrType(a1: AttrType, a2: AttrType): AttrType
-    requires lubOpt(a1.ty, a2.ty).Ok?
+  function lubAttrType(a1: AttrType, a2: AttrType, m: ValidationMode): AttrType
+    requires lubOpt(a1.ty, a2.ty, m).Ok?
   {
-    AttrType(lubOpt(a1.ty, a2.ty).value, a1.isRequired && a2.isRequired)
+    AttrType(lubOpt(a1.ty, a2.ty, m).value, a1.isRequired && a2.isRequired)
   }
 
   // This function produces a valid lub for any two maps, including ones that
   // are inconsistent. For example: the upper bound of { foo: Int } and
   // { foo: String } is the empty map type {}. This decision was made for the
   // sake of consistency with the Rust production implementation.
-  function lubRecordType(rt1: RecordType, rt2: RecordType): RecordType
+  function lubRecordType(rt1: RecordType, rt2: RecordType, m: ValidationMode): Result<RecordType>
     decreases Type.Record(rt1) , Type.Record(rt2) , 0
   {
     var attrs :=
-      map k | k in rt1.attrs.Keys && k in rt2.attrs.Keys && lubOpt(rt1.attrs[k].ty, rt2.attrs[k].ty).Ok? ::
-        lubAttrType(rt1.attrs[k], rt2.attrs[k]);
-    var openTag := if rt1.isOpen() || rt2.isOpen() || attrs.Keys != (rt1.attrs.Keys + rt2.attrs.Keys) then OpenAttributes else ClosedAttributes;
-    RecordType(attrs, openTag)
+      map k | k in rt1.attrs.Keys && k in rt2.attrs.Keys && lubOpt(rt1.attrs[k].ty, rt2.attrs[k].ty, m).Ok? ::
+        lubAttrType(rt1.attrs[k], rt2.attrs[k], m);
+    var widthSubtypingUsed := attrs.Keys != (rt1.attrs.Keys + rt2.attrs.Keys);
+    if m.isStrict() && widthSubtypingUsed
+    then Err(LubErr(Type.Record(rt1), Type.Record(rt2)))
+    else
+      var openTag := if rt1.isOpen() || rt2.isOpen() || widthSubtypingUsed  then OpenAttributes else ClosedAttributes;
+      Ok(RecordType(attrs, openTag))
   }
 
-  function lubRecordTypeSeq(rts: seq<RecordType>): Result<RecordType>
+  function lubRecordTypeSeq(rts: seq<RecordType>, m: ValidationMode): Result<RecordType>
   {
     if rts == [] then Err(EmptyLUB)
     else if |rts| == 1 then Ok(rts[0])
     else
-      var res :- lubRecordTypeSeq(rts[1..]);
-      Ok(lubRecordType(rts[0],res))
+      var res :- lubRecordTypeSeq(rts[1..],m);
+      lubRecordType(rts[0],res,m)
   }
 
-  function lubOpt(t1: Type, t2: Type): Result<Type>
+  function lubOpt(t1: Type, t2: Type, m: ValidationMode): Result<Type>
     decreases t1, t2 , 1
   {
     match (t1,t2) {
@@ -113,12 +123,15 @@ module validation.subtyping {
       case (String,String) => Ok(Type.String)
       case (Int,Int) => Ok(Type.Int)
       case (Bool(b1),Bool(b2)) => Ok(Type.Bool(lubBool(b1,b2)))
-      case (Entity(lub1),Entity(lub2)) => Ok(Type.Entity(lubEntity(lub1,lub2)))
+      case (Entity(lub1),Entity(lub2)) =>
+        var elub :- lubEntity(lub1,lub2, m);
+        Ok(Type.Entity(elub))
       case (Set(t11),Set(t12)) =>
-        var t :- lubOpt(t11,t12);
+        var t :- lubOpt(t11,t12, m);
         Ok(Type.Set(t))
       case(Record(rt1),Record(rt2)) =>
-        Ok(Type.Record(lubRecordType(rt1,rt2)))
+        var rtlub :- lubRecordType(rt1,rt2,m);
+        Ok(Type.Record(rtlub))
       case (Extension(e1),Extension(e2)) =>
         if e1 == e2 then Ok(Extension(e1))
         else Err(LubErr(t1,t2))
@@ -126,65 +139,74 @@ module validation.subtyping {
     }
   }
 
-  ghost predicate LubDefined(t1: Type,t2: Type) {
-    match lubOpt(t1,t2) {
+  ghost predicate LubDefined(t1: Type,t2: Type, m: ValidationMode) {
+    match lubOpt(t1,t2, m) {
       case Ok(_) => true
       case _ => false
     }
   }
 
-  function lub(t1: Type, t2: Type):  Type
-    requires LubDefined(t1,t2)
+  function lub(t1: Type, t2: Type, m: ValidationMode):  Type
+    requires LubDefined(t1,t2,m)
   {
-    match lubOpt(t1,t2) {
+    match lubOpt(t1,t2,m) {
       case Ok(t) => t
     }
   }
 
+  // Not true for Strict because AnyEntity </: AnyEntity.
   lemma SubtyRefl(t: Type)
-    ensures subty(t,t)
-  {}
-
-  lemma SubtyRecordTypeRefl(rt: RecordType)
-    ensures subtyRecordType(rt, rt)
+    ensures subty(t,t, ValidationMode.Permissive)
   {
-    forall k | k in rt.attrs.Keys ensures subtyAttrType(rt.attrs[k], rt.attrs[k]) {
-      SubtyRefl(rt.attrs[k].ty);
-    }
-  }
-
-  lemma SubtyRecordTypeTrans(rt1: RecordType, rt2: RecordType, rt3: RecordType)
-    requires subtyRecordType(rt1,rt2)
-    requires subtyRecordType(rt2,rt3)
-    ensures subtyRecordType(rt1,rt3)
-    decreases Type.Record(rt1) , Type.Record(rt2) , Type.Record(rt3) , 0
-  {
-    assert rt3.attrs.Keys <= rt1.attrs.Keys;
-    forall k | k in rt3.attrs.Keys
-      ensures subty(rt1.attrs[k].ty, rt3.attrs[k].ty)
-      ensures rt3.attrs[k].isRequired ==> rt1.attrs[k].isRequired
-    {
-      assert subty(rt1.attrs[k].ty, rt2.attrs[k].ty);
-      assert subty(rt2.attrs[k].ty, rt3.attrs[k].ty);
-      SubtyTrans(rt1.attrs[k].ty, rt2.attrs[k].ty, rt3.attrs[k].ty);
-    }
-  }
-
-  lemma SubtyTrans(t1: Type, t2: Type, t3: Type)
-    requires subty(t1,t2)
-    requires subty(t2,t3)
-    ensures subty(t1,t3)
-  {
-    match (t1,t2,t3) {
-      case (Record(rt1),Record(rt2),Record(rt3)) => SubtyRecordTypeTrans(rt1,rt2,rt3);
+    match t {
+      case Record(rt) => SubtyRecordTypeRefl(rt);
       case _ =>
     }
   }
 
+  lemma SubtyRecordTypeRefl(rt: RecordType)
+    ensures subtyRecordType(rt, rt, ValidationMode.Permissive)
+  {
+    forall k | k in rt.attrs.Keys ensures subtyAttrType(rt.attrs[k], rt.attrs[k], ValidationMode.Permissive) {
+      SubtyRefl(rt.attrs[k].ty);
+    }
+  }
+
+  lemma SubtyRecordTypeTrans(rt1: RecordType, rt2: RecordType, rt3: RecordType, m: ValidationMode)
+    requires subtyRecordType(rt1,rt2,m)
+    requires subtyRecordType(rt2,rt3,m)
+    ensures subtyRecordType(rt1,rt3,m)
+    decreases Type.Record(rt1) , Type.Record(rt2) , Type.Record(rt3) , 0
+  {
+    assert rt3.attrs.Keys <= rt1.attrs.Keys;
+    forall k | k in rt3.attrs.Keys
+      ensures subty(rt1.attrs[k].ty, rt3.attrs[k].ty, m)
+      ensures rt3.attrs[k].isRequired ==> rt1.attrs[k].isRequired
+    {
+      assert subty(rt1.attrs[k].ty, rt2.attrs[k].ty, m);
+      assert subty(rt2.attrs[k].ty, rt3.attrs[k].ty, m);
+      SubtyTrans(rt1.attrs[k].ty, rt2.attrs[k].ty, rt3.attrs[k].ty, m);
+    }
+  }
+
+  lemma SubtyTrans(t1: Type, t2: Type, t3: Type, m: ValidationMode)
+    requires subty(t1,t2,m)
+    requires subty(t2,t3,m)
+    ensures subty(t1,t3,m)
+    decreases t1, t2, t3
+  {
+    match (t1,t2,t3) {
+      case (Record(rt1),Record(rt2),Record(rt3)) => SubtyRecordTypeTrans(rt1,rt2,rt3,m);
+      case _ =>
+    }
+  }
+
+  // Not true for Strict mode because SubtyRefl is not true for Strict mode.
+  // Specifically, LUB(Never, AnyEntity) = AnyEntity, but  AnyEntity </: AnyEntity.
   lemma LubIsUB(t1: Type, t2: Type, t: Type)
-    requires lubOpt(t1,t2) == Ok(t)
-    ensures subty(t1,t)
-    ensures subty(t2,t)
+    requires lubOpt(t1,t2, ValidationMode.Permissive) == Ok(t)
+    ensures subty(t1,t, ValidationMode.Permissive)
+    ensures subty(t2,t, ValidationMode.Permissive)
   {
     match (t1,t2,t) {
       case (Never,_,_) => assert t2 == t; SubtyRefl(t);
@@ -197,25 +219,135 @@ module validation.subtyping {
       case(Record(rt1'),Record(rt2'),Record(rt')) =>
         assert rt'.attrs.Keys <= rt1'.attrs.Keys;
         assert rt'.attrs.Keys <= rt2'.attrs.Keys;
-        assert subty(Type.Record(rt1'),Type.Record(rt')) by {
+        assert subty(Type.Record(rt1'),Type.Record(rt'), ValidationMode.Permissive) by {
           forall k | k in rt'.attrs.Keys
-            ensures subtyAttrType(rt1'.attrs[k],rt'.attrs[k])
+            ensures subtyAttrType(rt1'.attrs[k],rt'.attrs[k], ValidationMode.Permissive)
           {
-            assert rt'.attrs[k] == lubAttrType(rt1'.attrs[k],rt2'.attrs[k]);
-            assert lubOpt(rt1'.attrs[k].ty,rt2'.attrs[k].ty) == Ok(rt'.attrs[k].ty);
+            assert rt'.attrs[k] == lubAttrType(rt1'.attrs[k],rt2'.attrs[k], ValidationMode.Permissive);
+            assert lubOpt(rt1'.attrs[k].ty,rt2'.attrs[k].ty, ValidationMode.Permissive) == Ok(rt'.attrs[k].ty);
             LubIsUB(rt1'.attrs[k].ty,rt2'.attrs[k].ty,rt'.attrs[k].ty);
           }
         }
-        assert subty(Type.Record(rt2'),Type.Record(rt')) by {
+        assert subty(Type.Record(rt2'),Type.Record(rt'),ValidationMode.Permissive) by {
           forall k | k in rt'.attrs.Keys
-            ensures subtyAttrType(rt2'.attrs[k],rt'.attrs[k])
+            ensures subtyAttrType(rt2'.attrs[k],rt'.attrs[k],ValidationMode.Permissive)
           {
-            assert rt'.attrs[k] == lubAttrType(rt1'.attrs[k],rt2'.attrs[k]);
-            assert lubOpt(rt1'.attrs[k].ty,rt2'.attrs[k].ty) == Ok(rt'.attrs[k].ty);
+            assert rt'.attrs[k] == lubAttrType(rt1'.attrs[k],rt2'.attrs[k], ValidationMode.Permissive);
+            assert lubOpt(rt1'.attrs[k].ty,rt2'.attrs[k].ty,ValidationMode.Permissive) == Ok(rt'.attrs[k].ty);
             LubIsUB(rt1'.attrs[k].ty,rt2'.attrs[k].ty,rt'.attrs[k].ty);
           }
         }
       case (Extension(n1),Extension(n2),Extension(n)) =>
+    }
+  }
+
+  lemma LubUndefUbUndef(t1 : Type, t2 : Type, t : Type, m: ValidationMode)
+    requires !LubDefined(t1, t2, m)
+    ensures !subty(t1, t, m) || !subty(t2, t, m)
+  {
+    match t {
+      case Never =>
+      case Int =>
+      case String =>
+      case Bool(b) =>
+      case Entity(e) =>
+      case Set(e) => {
+        if t1.Set? && t2.Set? {
+          LubUndefUbUndef(t1.ty, t2.ty, e, m);
+        }
+      }
+      case Record(rt) => {
+        match (t1, t2) {
+          case (Record(rt1), Record(rt2)) => {
+            if m.isStrict() {
+              // A strict mode record LUB might error for three reasons. The first two are discharged by Dafny.
+              assert lubRecordType(rt1, rt2, ValidationMode.Strict).Err?;
+              var attrs := map k | k in rt1.attrs.Keys && k in rt2.attrs.Keys && lubOpt(rt1.attrs[k].ty, rt2.attrs[k].ty, m).Ok? :: lubAttrType(rt1.attrs[k], rt2.attrs[k], m);
+              assert attrs.Keys != (rt1.attrs.Keys + rt2.attrs.Keys);
+              assert (exists k | k in rt1.attrs.Keys :: k !in rt2.attrs.Keys) ||
+                     (exists k | k in rt2.attrs.Keys :: k !in rt1.attrs.Keys) ||
+                     (exists k | k in rt1.attrs.Keys && k in rt2.attrs.Keys ::  !LubDefined(rt1.attrs[k].ty, rt2.attrs[k].ty, m));
+
+              // A strict mode record LUB might occur if there is an attribute
+              // which exists in both record with incompatible types.
+              if exists k | k in rt1.attrs.Keys && k in rt2.attrs.Keys :: !LubDefined(rt1.attrs[k].ty, rt2.attrs[k].ty, m) {
+                var k :| k in rt1.attrs.Keys && k in rt2.attrs.Keys && !LubDefined(rt1.attrs[k].ty, rt2.attrs[k].ty, m);
+
+                // If that key is not in supposed upper bound, then it clearly cannot be a subty of
+                if k in rt.attrs.Keys {
+                  var rt1k := rt1.attrs[k];
+                  var rt2k := rt2.attrs[k];
+                  var rtk := rt.attrs[k];
+                  assert !subty(rt1k.ty, rt.attrs[k].ty, m) ||
+                         !subty(rt2k.ty, rt.attrs[k].ty, m) by { LubUndefUbUndef(rt1k.ty, rt2k.ty, rtk.ty, m); }
+                  if !subty(rt1k.ty, rtk.ty, m) {
+                    assert (exists k' | k' in rt.attrs.Keys && k' in rt1.attrs.Keys :: !subtyAttrType(rt1.attrs[k'], rt.attrs[k'], m));
+                    assert !subty(t1, t, m);
+                  } else if !subty(rt2k.ty, rtk.ty, m) {
+                    assert (exists k' | k' in rt.attrs.Keys && k' in rt2.attrs.Keys :: !subtyAttrType(rt2.attrs[k'], rt.attrs[k'], m));
+                    assert !subty(t2, t, m);
+                  }
+                }
+              }
+
+            } else {
+              assert lubRecordType(rt1, rt2, ValidationMode.Permissive).Ok?;
+            }
+          }
+          case _ =>
+        }
+      }
+      case Extension(e) =>
+    }
+  }
+
+  lemma StrictSubtyIsStrict(t1: Type, t2: Type)
+    requires subty(t1, t2, ValidationMode.Strict)
+    ensures subty(t1, t2, ValidationMode.Permissive)
+  {
+    match (t1,t2) {
+      case (Record(rt1),Record(rt2)) =>  {
+        if(rt2.attrs.Keys <= rt1.attrs.Keys) {
+          if ! (forall k | k in rt2.attrs.Keys :: subtyAttrType(rt1.attrs[k], rt2.attrs[k], ValidationMode.Permissive)) {
+            assert exists k | k in rt2.attrs.Keys :: !subtyAttrType(rt1.attrs[k], rt2.attrs[k], ValidationMode.Permissive);
+            assert exists k | k in rt2.attrs.Keys :: !subtyAttrType(rt1.attrs[k], rt2.attrs[k], ValidationMode.Strict);
+          }
+        }
+      }
+      case _ =>
+    }
+  }
+
+  lemma StrictLubIsStrict(t1: Type, t2: Type)
+    requires LubDefined(t1, t2, ValidationMode.Strict)
+    ensures lubOpt(t1, t2, ValidationMode.Permissive) == lubOpt(t1, t2, ValidationMode.Strict)
+  {
+    match (t1,t2) {
+      case (Never,_) =>
+      case (_,Never) =>
+      case (Int,Int) =>
+      case (String,String) =>
+      case (Bool(b1),Bool(b2)) =>
+      case (Entity(e1),Entity(e2)) =>
+      case (Set(t1'),Set(t2')) =>
+      case (Record(rt1),Record(rt2)) => {
+        var slub_attrs :=
+          map k | k in rt1.attrs.Keys && k in rt2.attrs.Keys && lubOpt(rt1.attrs[k].ty, rt2.attrs[k].ty, ValidationMode.Strict).Ok? ::
+            lubAttrType(rt1.attrs[k], rt2.attrs[k], ValidationMode.Strict);
+        if slub_attrs.Keys == (rt1.attrs.Keys + rt2.attrs.Keys) {
+          var plub_attrs :=
+            map k | k in rt1.attrs.Keys && k in rt2.attrs.Keys && lubOpt(rt1.attrs[k].ty, rt2.attrs[k].ty, ValidationMode.Permissive).Ok? ::
+              lubAttrType(rt1.attrs[k], rt2.attrs[k], ValidationMode.Permissive);
+          assert plub_attrs == slub_attrs;
+
+          var openTag := if rt1.isOpen() || rt2.isOpen() then OpenAttributes else ClosedAttributes;
+          var lubrt := RecordType(slub_attrs, openTag);
+
+          assert lubRecordType(rt1, rt2, ValidationMode.Strict).value == lubrt;
+          assert lubRecordType(rt1, rt2, ValidationMode.Permissive).value == lubrt;
+        }
+      }
+      case (Extension(n1),Extension(n2)) =>
     }
   }
 }
