cedar-dafny/validation/thm/strict_soundness.dfy
@@ -1,0 +1,382 @@
+/*
+ * Copyright 2022-2023 Amazon.com, Inc. or its affiliates. All Rights Reserved.
+ *
+ * Licensed under the Apache License, Version 2.0 (the "License");
+ * you may not use this file except in compliance with the License.
+ * You may obtain a copy of the License at
+ *
+ *      https://www.apache.org/licenses/LICENSE-2.0
+ *
+ * Unless required by applicable law or agreed to in writing, software
+ * distributed under the License is distributed on an "AS IS" BASIS,
+ * WITHOUT WARRANTIES OR CONDITIONS OF ANY KIND, either express or implied.
+ * See the License for the specific language governing permissions and
+ * limitations under the License.
+ */
+
+include "../../def/all.dfy"
+include "../all.dfy"
+include "base.dfy"
+include "model.dfy"
+include "soundness.dfy"
+
+// This module contains the proof of soundness for strict typechecking.
+module validation.thm.strict_soundness {
+  import opened strict
+  import opened typechecker
+  import opened types
+  import opened subtyping
+  import opened base
+  import opened model
+  import opened soundness
+  import opened def.core
+  import opened def.engine
+  import opened ext
+
+  datatype StrictProof = StrictProof(
+    reqty: RequestType,
+    ets: EntityTypeStore,
+    acts: ActionStore
+  ) {
+
+    const P_TC := Typechecker(ets,acts,reqty, ValidationMode.Permissive)
+    const S_TC := Typechecker(ets,acts,reqty, ValidationMode.Strict)
+
+    lemma StrictCallArgs(e: Expr, args: seq<Expr>, tys: seq<Type>, effs: Effects)
+      decreases args, tys
+      requires |args| == |tys|
+      requires forall i | 0 <= i < |args| :: args[i] < e
+      requires S_TC.inferCallArgs(e, args, tys, effs).Ok?
+      ensures P_TC.inferCallArgs(e, args, tys, effs).Ok?
+    {
+      if args != [] {
+        var (t,effs') := S_TC.infer(args[0], effs).value;
+        assert P_TC.infer(args[0], effs) == Ok((t, effs')) by { StrictTypecheckingIsStrict(args[0], effs); }
+
+        assert subty(t, tys[0], ValidationMode.Strict);
+        assert subty(t, tys[0], ValidationMode.Permissive) by { StrictSubtyIsStrict(t, tys[0]); }
+
+        assert S_TC.inferCallArgs(e, args[1..], tys[1..], effs).Ok?;
+        assert P_TC.inferCallArgs(e, args[1..], tys[1..], effs).Ok? by { StrictCallArgs(e, args[1..], tys[1..], effs); }
+      }
+    }
+
+    lemma StrictCall(name: base.Name, args: seq<Expr>, effs: Effects)
+      decreases args
+      requires S_TC.infer(Call(name, args), effs).Ok?
+      ensures P_TC.infer(Call(name, args), effs) == S_TC.infer(Call(name, args), effs)
+    {
+      var ty := extFunTypes[name];
+      assert S_TC.inferCallArgs(Call(name, args), args, ty.args, effs).Ok?;
+      assert P_TC.inferCallArgs(Call(name, args), args, ty.args, effs).Ok? by { StrictCallArgs(Call(name, args), args, ty.args, effs); }
+    }
+
+    lemma StrictSetElems(e: Expr, es: seq<Expr>, effs: Effects)
+      decreases es
+      requires forall i | 0 <= i < |es| :: es[i] < e
+      requires S_TC.inferSet(e, es, effs).Ok?
+      ensures P_TC.inferSet(e, es, effs) == S_TC.inferSet(e, es, effs)
+    {
+      if es != [] {
+        var (t, effs') := S_TC.infer(es[0], effs).value;
+        assert P_TC.infer(es[0], effs) == Ok((t, effs')) by { StrictTypecheckingIsStrict(es[0], effs); }
+
+        var t1 := S_TC.inferSet(e, es[1..], effs).value;
+        assert P_TC.inferSet(e, es[1..], effs) == Ok(t1) by { StrictSetElems(e, es[1..], effs); }
+
+        var lub := lub(t, t1, ValidationMode.Strict);
+        assert lubOpt(t, t1, ValidationMode.Permissive) == Ok(lub) by { StrictLubIsStrict(t, t1); }
+      }
+    }
+
+    lemma StrictNot(e: Expr, effs: Effects)
+      decreases UnaryApp(Not, e), 0
+      requires S_TC.infer(UnaryApp(Not, e), effs).Ok?
+      ensures P_TC.infer(UnaryApp(Not, e), effs) == S_TC.infer(UnaryApp(Not, e), effs)
+    {
+      assert P_TC.inferBoolType(e, effs) == S_TC.inferBoolType(e, effs) by {
+        StrictTypecheckingIsStrict(e, effs);
+      }
+    }
+
+    lemma StrictArith1(o: UnaryOp, e: Expr, effs: Effects)
+      decreases UnaryApp(o, e), 0
+      requires o.Neg? || o.MulBy?
+      requires S_TC.infer(UnaryApp(o, e), effs).Ok?
+      ensures P_TC.infer(UnaryApp(o, e), effs) == S_TC.infer(UnaryApp(o, e), effs)
+    {
+      assert P_TC.ensureIntType(e, effs).Ok? by {
+        assert S_TC.ensureIntType(e, effs).Ok?;
+        StrictTypecheckingIsStrict(e, effs);
+      }
+    }
+
+    lemma StrictLike(p: Pattern, e: Expr, effs: Effects)
+      decreases UnaryApp(Like(p), e), 0
+      requires S_TC.infer(UnaryApp(Like(p), e), effs).Ok?
+      ensures P_TC.infer(UnaryApp(Like(p), e), effs) == S_TC.infer(UnaryApp(Like(p), e), effs)
+    {
+      assert P_TC.ensureStringType(e, effs).Ok? by {
+        assert S_TC.ensureStringType(e, effs).Ok?;
+        StrictTypecheckingIsStrict(e, effs);
+      }
+    }
+
+    lemma StrictArith2Ineq(o: BinaryOp, e1: Expr, e2: Expr, effs: Effects)
+      decreases BinaryApp(o, e1, e2), 0
+      requires o.Add? || o.Sub? || o.Less? || o.LessEq?
+      requires S_TC.infer(BinaryApp(o, e1, e2), effs).Ok?
+      ensures P_TC.infer(BinaryApp(o, e1, e2), effs) == S_TC.infer(BinaryApp(o, e1, e2), effs)
+    {
+      assert P_TC.ensureIntType(e1, effs).Ok? by {
+        assert S_TC.ensureIntType(e1, effs).Ok?;
+        StrictTypecheckingIsStrict(e1, effs);
+      }
+      assert P_TC.ensureIntType(e2, effs).Ok? by {
+        assert S_TC.ensureIntType(e2, effs).Ok?;
+        StrictTypecheckingIsStrict(e2, effs);
+      }
+    }
+
+    lemma StrictLubRecordTypeSeq(rts: seq<RecordType>)
+      requires lubRecordTypeSeq(rts, ValidationMode.Strict).Ok?
+      ensures lubRecordTypeSeq(rts, ValidationMode.Permissive) == lubRecordTypeSeq(rts, ValidationMode.Strict)
+    {
+      assert rts != [];
+      if |rts| != 1 {
+        var tailLub := lubRecordTypeSeq(rts[1..], ValidationMode.Strict).value;
+        assert lubRecordTypeSeq(rts[1..], ValidationMode.Permissive) == Ok(tailLub) by { StrictLubRecordTypeSeq(rts[1..]); }
+
+        assert lubRecordType(rts[0], tailLub, ValidationMode.Strict) == lubRecordType(rts[0], tailLub, ValidationMode.Permissive) by {
+          StrictLubIsStrict(Type.Record(rts[0]), Type.Record(tailLub));
+        }
+      }
+    }
+
+    lemma StrictGetLubRecordType(lub: EntityLUB)
+      requires ets.getLubRecordType(lub, ValidationMode.Strict).Ok?
+      ensures ets.getLubRecordType(lub, ValidationMode.Permissive) == ets.getLubRecordType(lub, ValidationMode.Strict)
+    {
+      if lub.AnyEntity? || exists et <- lub.tys :: isAction(et) {
+        assert ets.getLubRecordType(lub, ValidationMode.Permissive).Ok?;
+      } else {
+        assert forall et <- lub.tys :: et in ets.types;
+        def.util.EntityTypeLeqIsTotalOrder();
+        var lubSeq := def.util.SetToSortedSeq(lub.tys,def.util.EntityTypeLeq);
+        var s := seq (|lubSeq|, i requires 0 <= i < |lubSeq| => ets.types[lubSeq[i]]);
+        assert s != [];
+        assert lubRecordTypeSeq(s, ValidationMode.Strict) == lubRecordTypeSeq(s, ValidationMode.Permissive) by {
+          assert ets.getLubRecordType(lub, ValidationMode.Strict).Ok?;
+          StrictLubRecordTypeSeq(s);
+        }
+      }
+    }
+
+    lemma StrictHasAttr(e: Expr, l: Attr, effs: Effects)
+      decreases HasAttr(e, l), 0
+      requires S_TC.infer(HasAttr(e, l), effs).Ok?
+      ensures P_TC.infer(HasAttr(e, l), effs) == S_TC.infer(HasAttr(e, l), effs)
+    {
+      var ret := S_TC.inferRecordEntityType(e, effs).value;
+      assert P_TC.inferRecordEntityType(e, effs) == Ok(ret) by { StrictTypecheckingIsStrict(e, effs); }
+
+      match ret {
+        case Record(rt) =>
+        case Entity(lub) =>
+          if ets.isAttrPossible(lub,l) {
+            var rt := ets.getLubRecordType(lub, ValidationMode.Strict).value;
+            assert ets.getLubRecordType(lub, ValidationMode.Permissive) == Ok(rt) by { StrictGetLubRecordType(lub); }
+          }
+      }
+    }
+
+    lemma StrictGetAttr(e: Expr, l: Attr, effs:Effects)
+      decreases GetAttr(e, l), 0
+      requires S_TC.infer(GetAttr(e, l), effs).Ok?
+      ensures P_TC.infer(GetAttr(e, l), effs) == S_TC.infer(GetAttr(e, l), effs)
+    {
+      var ret := S_TC.inferRecordEntityType(e, effs).value;
+      assert P_TC.inferRecordEntityType(e, effs) == Ok(ret) by { StrictTypecheckingIsStrict(e, effs); }
+
+      match ret {
+        case Record(rt) =>
+        case Entity(lub) => {
+          var rt := ets.getLubRecordType(lub, ValidationMode.Strict).value;
+          assert ets.getLubRecordType(lub, ValidationMode.Permissive) == Ok(rt) by { StrictGetLubRecordType(lub); }
+        }
+      }
+    }
+
+    lemma StrictIf(g: Expr, t: Expr, e: Expr, effs: Effects)
+      decreases If(g, t, e), 0
+      requires S_TC.infer(If(g, t, e), effs).Ok?
+      ensures P_TC.infer(If(g, t, e), effs) == S_TC.infer(If(g, t, e), effs)
+    {
+      var (gt, ge) := S_TC.inferBoolType(g, effs).value;
+      assert P_TC.inferBoolType(g, effs) == Ok((gt, ge)) by { StrictTypecheckingIsStrict(g, effs); }
+
+      match gt {
+        case True => {
+          var (tt, te) := S_TC.infer(t, effs.union(ge)).value;
+          assert P_TC.infer(t, effs.union(ge)) == Ok((tt, te)) by { StrictTypecheckingIsStrict(t, effs.union(ge)); }
+        }
+        case False => {
+          var (et, ee) := S_TC.infer(e, effs).value;
+          assert P_TC.infer(e, effs) == Ok((et, ee)) by { StrictTypecheckingIsStrict(e, effs); }
+        }
+        case Bool => {
+          var (tt, te) := S_TC.infer(t, effs.union(ge)).value;
+          assert P_TC.infer(t, effs.union(ge)) == Ok((tt, te)) by { StrictTypecheckingIsStrict(t, effs.union(ge)); }
+
+          var (et, ee) := S_TC.infer(e, effs).value;
+          assert P_TC.infer(e, effs) == Ok((et, ee)) by { StrictTypecheckingIsStrict(e, effs); }
+
+          var lub := lub(tt, et, ValidationMode.Strict);
+          assert lubOpt(tt, et, ValidationMode.Permissive) == Ok(lub) by { StrictLubIsStrict(tt, et); }
+        }
+      }
+    }
+
+    lemma StrictEq(e1: Expr, e2: Expr, effs: Effects)
+      decreases BinaryApp(BinaryOp.Eq, e1, e2), 0
+      requires S_TC.infer(BinaryApp(BinaryOp.Eq, e1, e2), effs).Ok?
+      ensures P_TC.infer(BinaryApp(BinaryOp.Eq, e1, e2), effs) == S_TC.infer(BinaryApp(BinaryOp.Eq, e1, e2), effs)
+    {
+      var (t1, effs1) := S_TC.infer(e1, effs).value;
+      assert  P_TC.infer(e1, effs) == Ok((t1, effs1)) by { StrictTypecheckingIsStrict(e1, effs); }
+
+      var (t2, effs2) := S_TC.infer(e2, effs).value;
+      assert P_TC.infer(e2, effs) == Ok((t2, effs2)) by { StrictTypecheckingIsStrict(e2, effs); }
+    }
+
+    lemma StrictContainsAnyAll(o: BinaryOp, e1: Expr, e2: Expr, effs: Effects)
+      decreases BinaryApp(o, e1, e2), 0
+      requires o.ContainsAny? || o.ContainsAll?
+      requires S_TC.infer(BinaryApp(o, e1, e2), effs).Ok?
+      ensures P_TC.infer(BinaryApp(o, e1, e2), effs) == S_TC.infer(BinaryApp(o, e1, e2), effs)
+    {
+      var t1 := S_TC.inferSetType(e1, effs).value;
+      assert  P_TC.inferSetType(e1, effs) == Ok(t1) by { StrictTypecheckingIsStrict(e1, effs); }
+
+      var t2 := S_TC.inferSetType(e2, effs).value;
+      assert P_TC.inferSetType(e2, effs) == Ok(t2) by { StrictTypecheckingIsStrict(e2, effs); }
+    }
+
+    lemma StrictContains(e1: Expr, e2: Expr, effs: Effects)
+      decreases BinaryApp(BinaryOp.Contains, e1, e2), 0
+      requires S_TC.infer(BinaryApp(BinaryOp.Contains, e1, e2), effs).Ok?
+      ensures P_TC.infer(BinaryApp(BinaryOp.Contains, e1, e2), effs) == S_TC.infer(BinaryApp(BinaryOp.Contains, e1, e2), effs)
+    {
+      var t1 := S_TC.inferSetType(e1, effs).value;
+      assert  P_TC.inferSetType(e1, effs) == Ok(t1) by { StrictTypecheckingIsStrict(e1, effs); }
+
+      var (t2, effs2) := S_TC.infer(e2, effs).value;
+      assert P_TC.infer(e2, effs) == Ok((t2, effs2)) by { StrictTypecheckingIsStrict(e2, effs); }
+    }
+
+    lemma StrictIn(e1: Expr, e2: Expr, effs: Effects)
+      decreases BinaryApp(BinaryOp.In, e1, e2), 0
+      requires S_TC.infer(BinaryApp(BinaryOp.In, e1, e2), effs).Ok?
+      ensures P_TC.infer(BinaryApp(BinaryOp.In, e1, e2), effs) == S_TC.infer(BinaryApp(BinaryOp.In, e1, e2), effs)
+    {
+      assert S_TC.ensureEntityType(e1,effs).Ok?;
+      assert P_TC.ensureEntityType(e1,effs).Ok? by { StrictTypecheckingIsStrict(e1, effs); }
+
+      assert S_TC.ensureEntitySetType(e2,effs).Ok?;
+      assert P_TC.ensureEntitySetType(e2,effs).Ok? by { StrictTypecheckingIsStrict(e2, effs); }
+
+      var (t2, effs') := S_TC.infer(e2,effs).value;
+      assert P_TC.infer(e2, effs) == Ok((t2, effs')) by { StrictTypecheckingIsStrict(e2, effs); }
+    }
+
+    lemma StrictAnd(e1: Expr, e2: Expr, effs: Effects)
+      decreases And(e1, e2), 0
+      requires S_TC.infer(And(e1, e2), effs).Ok?
+      ensures P_TC.infer(And(e1, e2), effs) == S_TC.infer(And(e1, e2), effs)
+    {
+      var (bt1,effs1) := S_TC.inferBoolType(e1,effs).value;
+      assert P_TC.inferBoolType(e1,effs) == Ok((bt1, effs1)) by { StrictTypecheckingIsStrict(e1, effs); }
+
+      match bt1 {
+        case True => {
+          var (bt2,effs2) := S_TC.inferBoolType(e2,effs.union(effs1)).value;
+          assert P_TC.inferBoolType(e2,effs.union(effs1)) == Ok((bt2, effs2)) by { StrictTypecheckingIsStrict(e2, effs.union(effs1)); }
+        }
+        case False =>
+        case Bool => {
+          var (bt2,effs2) := S_TC.inferBoolType(e2,effs.union(effs1)).value;
+          assert P_TC.inferBoolType(e2,effs.union(effs1)) == Ok((bt2, effs2)) by { StrictTypecheckingIsStrict(e2, effs.union(effs1)); }
+        }
+      }
+    }
+
+    lemma StrictOr(e1: Expr, e2: Expr, effs: Effects)
+      decreases Or(e1, e2), 0
+      requires S_TC.infer(Or(e1, e2), effs).Ok?
+      ensures P_TC.infer(Or(e1, e2), effs) == S_TC.infer(Or(e1, e2), effs)
+    {
+      var (bt1,effs1) := S_TC.inferBoolType(e1,effs).value;
+      assert P_TC.inferBoolType(e1,effs) == Ok((bt1, effs1)) by { StrictTypecheckingIsStrict(e1, effs); }
+
+      match bt1 {
+        case True =>
+        case False => {
+          var (bt2,effs2) := S_TC.inferBoolType(e2,effs).value;
+          assert P_TC.inferBoolType(e2,effs) == Ok((bt2, effs2)) by { StrictTypecheckingIsStrict(e2, effs); }
+        }
+        case Bool => {
+          var (bt2,effs2) := S_TC.inferBoolType(e2,effs).value;
+          assert P_TC.inferBoolType(e2,effs) == Ok((bt2, effs2)) by { StrictTypecheckingIsStrict(e2, effs); }
+        }
+      }
+    }
+
+    lemma StrictRecord(e: Expr, r: seq<(Attr,Expr)>, effs: Effects)
+      decreases r
+      requires forall i | 0 <= i < |r| :: r[i] < e
+      requires S_TC.inferRecord(e, r, effs).Ok?
+      ensures P_TC.inferRecord(e, r, effs) == S_TC.inferRecord(e, r, effs)
+    {
+      reveal S_TC.inferRecord();
+      if r != [] {
+        var (t,effs') := S_TC.infer(r[0].1,effs).value;
+        assert P_TC.infer(r[0].1, effs) == Ok((t, effs')) by {StrictTypecheckingIsStrict(r[0].1, effs); }
+
+        var m := S_TC.inferRecord(e, r[1..], effs).value;
+        assert P_TC.inferRecord(e, r[1..], effs) == Ok(m) by { StrictRecord(e, r[1..], effs); }
+      }
+    }
+
+    lemma StrictTypecheckingIsStrict(e: Expr, effs: Effects)
+      decreases e, 1
+      requires S_TC.infer(e, effs).Ok?
+      ensures P_TC.infer(e, effs) == S_TC.infer(e, effs)
+    {
+      match e {
+        case PrimitiveLit(p) =>
+        case Var(x) =>
+        case If(e',e1,e2) => StrictIf(e', e1, e2, effs);
+        case And(e1,e2) => StrictAnd(e1, e2, effs);
+        case Or(e1,e2) => StrictOr(e1, e2, effs);
+        case UnaryApp(Not,e') => StrictNot(e', effs);
+        case UnaryApp(Neg,e') => StrictArith1(Neg, e', effs);
+        case UnaryApp(MulBy(i),e') => StrictArith1(MulBy(i), e', effs);
+        case UnaryApp(Like(p),e') => StrictLike(p, e', effs);
+        case BinaryApp(Eq,e1,e2) => StrictEq(e1, e2, effs);
+        case BinaryApp(Less,e1,e2) => StrictArith2Ineq(Less, e1, e2, effs);
+        case BinaryApp(LessEq,e1,e2) => StrictArith2Ineq(LessEq, e1, e2, effs);
+        case BinaryApp(Add,e1,e2) => StrictArith2Ineq(Add, e1, e2, effs);
+        case BinaryApp(Sub,e1,e2) => StrictArith2Ineq(Sub, e1, e2, effs);
+        case BinaryApp(In,e1,e2) => StrictIn(e1, e2, effs);
+        case BinaryApp(ContainsAny,e1,e2) => StrictContainsAnyAll(ContainsAny, e1, e2, effs);
+        case BinaryApp(ContainsAll,e1,e2) => StrictContainsAnyAll(ContainsAll, e1, e2, effs);
+        case BinaryApp(Contains,e1,e2) => StrictContains(e1, e2, effs);
+        case Record(es) => StrictRecord(e, es, effs);
+        case Set(es) => StrictSetElems(e, es, effs);
+        case GetAttr(e',l) => StrictGetAttr(e', l, effs);
+        case HasAttr(e',l) => StrictHasAttr(e', l, effs);
+        case Call(name,es) => StrictCall(name, es, effs);
+      }
+    }
+  }
+}
